restore the elaborator (as is)

src/cddl/spec/CDDL.Spec.AST.Elab.fst
@@ -1,8 +1,8 @@
-module CDDL.Interpreter.Elab
-include CDDL.Interpreter.AST
-module Spec = CDDL.Spec
+module CDDL.Spec.AST.Elab
+include CDDL.Spec.AST.Base
+module Cbor = CBOR.Spec.API.Type
+module Spec = CDDL.Spec.All
 module U64 = FStar.UInt64
-module MapSpec = CDDL.Spec.MapGroupGen
 
 noeq
 type result (t: Type) =
@@ -43,7 +43,7 @@ let rec map_group_is_productive_correct
     RSuccess? (map_group_is_productive g)
   ))
   (ensures (
-    MapSpec.map_group_is_productive (map_group_sem env g)
+    Spec.map_group_is_productive (map_group_sem env g)
   ))
 = match g with
   | GOneOrMore g' ->
@@ -55,6 +55,64 @@ let rec map_group_is_productive_correct
     if RSuccess? (map_group_is_productive g1)
     then map_group_is_productive_correct env g1
     else map_group_is_productive_correct env g2
+  | _ -> ()
+
+[@@ sem_attr]
+let rec apply_map_group_det_empty_fail
+  (g: group NMapGroup)
+: Tot (result bool)
+= match g with
+  | GOneOrMore _ -> RFailure "apply_map_group_det_empty_fail: GOneOrMore"
+  | GAlwaysFalse
+  | GMapElem _ true _ _
+  | GMapElem _ _ (TElem (ELiteral _)) _ -> RSuccess true
+  | GMapElem _ _ _ _ -> RFailure "apply_map_group_det_empty_fail: GMapElem"
+  | GNop -> RSuccess false
+  | GZeroOrOne _
+  | GZeroOrMore _ -> RFailure "this should be `RSuccess false`"
+  | GChoice g1 g2 ->
+    begin match apply_map_group_det_empty_fail g1 with
+    | RSuccess true -> apply_map_group_det_empty_fail g2
+    | res -> res
+    end
+  | GConcat g1 g2 ->
+    begin match apply_map_group_det_empty_fail g1 with
+    | RSuccess false -> apply_map_group_det_empty_fail g2
+    | res -> res
+    end
+
+let rec apply_map_group_det_empty_fail_correct
+  (env: sem_env)
+  (g: group NMapGroup)
+: Lemma
+  (requires (
+    group_bounded NMapGroup env.se_bound g /\
+    RSuccess? (apply_map_group_det_empty_fail g)
+  ))
+  (ensures (
+    match apply_map_group_det_empty_fail g, Spec.apply_map_group_det (map_group_sem env g) Cbor.cbor_map_empty with
+    | RSuccess true, Spec.MapGroupFail
+    | RSuccess false, Spec.MapGroupDet _ _ -> True
+    | _ -> False
+  ))
+= match g with
+  | GChoice g1 g2 ->
+    apply_map_group_det_empty_fail_correct env g1;
+    begin match apply_map_group_det_empty_fail g1 with
+    | RSuccess true -> apply_map_group_det_empty_fail_correct env g2
+    | _ -> ()
+    end
+  | GConcat g1 g2 ->
+    apply_map_group_det_empty_fail_correct env g1;
+    begin match apply_map_group_det_empty_fail g1 with
+    | RSuccess false ->
+      let Spec.MapGroupDet _ rem = Spec.apply_map_group_det (map_group_sem env g1) Cbor.cbor_map_empty in
+      assert (Cbor.cbor_map_equal rem Cbor.cbor_map_empty);
+      apply_map_group_det_empty_fail_correct env g2
+    | _ -> ()
+    end
+  | GMapElem _ cut (TElem (ELiteral k)) v ->
+    Spec.apply_map_group_det_match_item_for cut (eval_literal k) (typ_sem env v) Cbor.cbor_map_empty
   | _ -> ()
 
 [@@ sem_attr]
@@ -174,7 +232,7 @@ and rewrite_group_correct
     let t' = rewrite_group fuel kind t in
     group_bounded kind env.se_bound t' /\
     begin match kind with
-    | NArrayGroup -> Spec.array_group3_equiv (array_group_sem env t) (array_group_sem env t')
+    | NArrayGroup -> Spec.array_group_equiv (array_group_sem env t) (array_group_sem env t')
     | NMapGroup -> map_group_sem env t == map_group_sem env t'
     | _ -> True
     end
@@ -200,7 +258,7 @@ and rewrite_group_correct
     rewrite_group_correct env fuel' t2;
     rewrite_group_correct env fuel' (GConcat t1' t2');
     begin match kind with
-    | NArrayGroup -> Spec.array_group3_concat_equiv (array_group_sem env t1) (array_group_sem env t1') (array_group_sem env t2) (array_group_sem env t2')
+    | NArrayGroup -> Spec.array_group_concat_equiv (array_group_sem env t1) (array_group_sem env t1') (array_group_sem env t2) (array_group_sem env t2')
     | _ -> ()
     end
   | GChoice GAlwaysFalse g -> rewrite_group_correct env fuel' g
@@ -214,13 +272,13 @@ and rewrite_group_correct
     rewrite_group_correct env fuel' t2;
     rewrite_group_correct env fuel' (GChoice t1' t2')
   | GZeroOrMore (GMapElem sq cut (TElem (ELiteral key)) value) ->
-    MapSpec.map_group_zero_or_more_map_group_match_item_for cut (eval_literal key) (typ_sem env value);
+    Spec.map_group_zero_or_more_map_group_match_item_for cut (eval_literal key) (typ_sem env value);
     rewrite_group_correct env fuel' (GZeroOrOne (GMapElem sq cut (TElem (ELiteral key)) value))
   | GZeroOrMore (GChoice (GMapElem sq cut key value) g') ->
     if RSuccess? (map_group_is_productive g')
     then begin
       map_group_is_productive_correct env g';
-      MapSpec.map_group_zero_or_more_choice (MapSpec.map_group_match_item cut (typ_sem env key) (typ_sem env value)) (map_group_sem env g');
+      Spec.map_group_zero_or_more_choice (Spec.map_group_match_item cut (typ_sem env key) (typ_sem env value)) (map_group_sem env g');
       rewrite_group_correct env fuel' (GConcat (GZeroOrMore (GMapElem sq cut key value)) (GZeroOrMore g'))
     end
   | GZeroOrOne g1 ->
@@ -230,7 +288,7 @@ and rewrite_group_correct
     let g2 = rewrite_group fuel' kind g1 in
     rewrite_group_correct env fuel' (GZeroOrMore g2);
     begin match kind with
-    | NArrayGroup -> Spec.array_group3_zero_or_more_equiv (array_group_sem env g1) (array_group_sem env g2)
+    | NArrayGroup -> Spec.array_group_zero_or_more_equiv (array_group_sem env g1) (array_group_sem env g2)
     | _ -> ()
     end
   | GOneOrMore g1 ->
@@ -238,16 +296,16 @@ and rewrite_group_correct
     let g2 = rewrite_group fuel' kind g1 in
     rewrite_group_correct env fuel' (GOneOrMore g2);
     begin match kind with
-    | NArrayGroup -> Spec.array_group3_zero_or_more_equiv (array_group_sem env g1) (array_group_sem env g2)
+    | NArrayGroup -> Spec.array_group_zero_or_more_equiv (array_group_sem env g1) (array_group_sem env g2)
     | _ -> ()
     end
   | GArrayElem sq ty ->
     rewrite_typ_correct env fuel' ty;
-    Spec.array_group3_item_equiv (typ_sem env ty) (typ_sem env (rewrite_typ fuel' ty))
+    Spec.array_group_item_equiv (typ_sem env ty) (typ_sem env (rewrite_typ fuel' ty))
   | GMapElem sq cut key value ->
     rewrite_typ_correct env fuel' key;
     rewrite_typ_correct env fuel' value;
-    MapSpec.map_group_match_item_ext cut (typ_sem env key) (typ_sem env value) (typ_sem env (rewrite_typ fuel' key)) (typ_sem env (rewrite_typ fuel' value))
+    Spec.map_group_match_item_ext cut (typ_sem env key) (typ_sem env value) (typ_sem env (rewrite_typ fuel' key)) (typ_sem env (rewrite_typ fuel' value))
   | GAlwaysFalse
   | GNop
   | GDef _ _ -> ()
@@ -266,11 +324,11 @@ let destruct_group
 
 let maybe_close_array_group_concat
   (close: bool)
-  (a1 a2: Spec.array_group3 None)
+  (a1 a2: Spec.array_group None)
 : Lemma
-  (Spec.array_group3_equiv
-    (Spec.maybe_close_array_group (Spec.array_group3_concat a1 a2) close)
-    (Spec.array_group3_concat a1 (Spec.maybe_close_array_group a2 close))
+  (Spec.array_group_equiv
+    (Spec.maybe_close_array_group (Spec.array_group_concat a1 a2) close)
+    (Spec.array_group_concat a1 (Spec.maybe_close_array_group a2 close))
   )
 = ()
 
@@ -281,7 +339,7 @@ let array_group_sem_destruct_group
   (let (g1, g2) = destruct_group g in
     group_bounded _ e.se_bound g1 /\
     group_bounded _ e.se_bound g2 /\
-    array_group_sem e g `Spec.array_group3_equiv` (array_group_sem e g1 `Spec.array_group3_concat` array_group_sem e g2)
+    array_group_sem e g `Spec.array_group_equiv` (array_group_sem e g1 `Spec.array_group_concat` array_group_sem e g2)
   )
 = ()
 
@@ -293,8 +351,8 @@ let maybe_close_array_group_sem_destruct_group
   (let (g1, g2) = destruct_group g in
     group_bounded _ e.se_bound g1 /\
     group_bounded _ e.se_bound g2 /\
-    Spec.maybe_close_array_group (array_group_sem e g) close `Spec.array_group3_equiv`
-      (array_group_sem e g1 `Spec.array_group3_concat` Spec.maybe_close_array_group (array_group_sem e g2) close)
+    Spec.maybe_close_array_group (array_group_sem e g) close `Spec.array_group_equiv`
+      (array_group_sem e g1 `Spec.array_group_concat` Spec.maybe_close_array_group (array_group_sem e g2) close)
   )
   [SMTPat (Spec.maybe_close_array_group (array_group_sem e g) close)]
 = ()
@@ -303,20 +361,20 @@ let maybe_close_array_group_sem_destruct_group
 let array_group_concat_elem_same_disjoint
   (close: bool)
   (t1 t2: Spec.typ)
-  (a1 a2: Spec.array_group3 None)
+  (a1 a2: Spec.array_group None)
 : Lemma
   (requires
     Spec.typ_equiv t1 t2
   )
-  (ensures (Spec.array_group3_disjoint (Spec.maybe_close_array_group a1 close) (Spec.maybe_close_array_group a2 close) ==>
-    Spec.array_group3_disjoint
-      (Spec.maybe_close_array_group (Spec.array_group3_concat (Spec.array_group3_item t1) a1) close)
-      (Spec.maybe_close_array_group (Spec.array_group3_concat (Spec.array_group3_item t2) a2) close)
+  (ensures (Spec.array_group_disjoint (Spec.maybe_close_array_group a1 close) (Spec.maybe_close_array_group a2 close) ==>
+    Spec.array_group_disjoint
+      (Spec.maybe_close_array_group (Spec.array_group_concat (Spec.array_group_item t1) a1) close)
+      (Spec.maybe_close_array_group (Spec.array_group_concat (Spec.array_group_item t2) a2) close)
   ))
-= maybe_close_array_group_concat close (Spec.array_group3_item t1) a1;
-  maybe_close_array_group_concat close (Spec.array_group3_item t1) a2
+= maybe_close_array_group_concat close (Spec.array_group_item t1) a1;
+  maybe_close_array_group_concat close (Spec.array_group_item t1) a2
 
-#push-options "--admit_smt_queries true" // "--z3rlimit 128 --query_stats --split_queries always --fuel 4 --ifuel 8"
+#push-options "--z3rlimit 128 --query_stats --split_queries always --fuel 4 --ifuel 8"
 
 #restart-solver
 [@@"opaque_to_smt"]
@@ -368,25 +426,26 @@ let rec typ_disjoint
     else RSuccess ()
   | TElem (ELiteral (LInt ty _)), TElem EUInt
   | TElem EUInt, TElem (ELiteral (LInt ty _)) ->
-    if ty = CBOR.Spec.cbor_major_type_uint64
+    if ty = Cbor.cbor_major_type_uint64
     then RFailure "typ_disjoint: uint64"
     else RSuccess ()
   | TElem (ELiteral (LInt ty _)), TElem ENInt
   | TElem ENInt, TElem (ELiteral (LInt ty _)) ->
-    if ty = CBOR.Spec.cbor_major_type_neg_int64
+    if ty = Cbor.cbor_major_type_neg_int64
     then RFailure "typ_disjoint: neg_int64"
     else RSuccess ()
   | TElem (ELiteral (LString ty _)), TElem EByteString
   | TElem EByteString, TElem (ELiteral (LString ty _)) ->
-    if ty = CBOR.Spec.cbor_major_type_byte_string
+    if ty = Cbor.cbor_major_type_byte_string
     then RFailure "typ_disjoint: byte string"
     else RSuccess ()
   | TElem (ELiteral (LString ty _)), TElem ETextString
   | TElem ETextString, TElem (ELiteral (LString ty _)) ->
-    if ty = CBOR.Spec.cbor_major_type_text_string
+    if ty = Cbor.cbor_major_type_text_string
     then RFailure "typ_disjoint: text string"
     else RSuccess ()
-  | TElem e1, TElem e2 ->
+  | TElem (ELiteral (LString ty1 s1)), TElem (ELiteral (LString ty2 s2)) ->
+    byte_seq_of_ascii_string_diff s1 s2;
     RSuccess ()
   | TElem _, _
   | _, TElem _ -> RSuccess ()
@@ -394,8 +453,8 @@ let rec typ_disjoint
   | TMap _, _
   | _, TMap _ -> RSuccess ()
   | TArray a1, TArray a2 ->
-    Spec.array3_close_array_group (array_group_sem e.e_sem_env a1);
-    Spec.array3_close_array_group (array_group_sem e.e_sem_env a2);
+    Spec.array_close_array_group (array_group_sem e.e_sem_env a1);
+    Spec.array_close_array_group (array_group_sem e.e_sem_env a2);
     array_group_disjoint e fuel' true a1 a2
   | TArray _, _
   | _, TArray _ -> RSuccess ()
@@ -410,7 +469,7 @@ and array_group_disjoint
 : Pure (result unit)
     (requires True)
     (ensures fun r ->
-      RSuccess? r ==> Spec.array_group3_disjoint (Spec.maybe_close_array_group (array_group_sem e.e_sem_env a1) close) (Spec.maybe_close_array_group (array_group_sem e.e_sem_env a2) close)
+      RSuccess? r ==> Spec.array_group_disjoint (Spec.maybe_close_array_group (array_group_sem e.e_sem_env a1) close) (Spec.maybe_close_array_group (array_group_sem e.e_sem_env a2) close)
     )
     (decreases fuel)
 = let a10 = a1 in
@@ -440,8 +499,8 @@ and array_group_disjoint
   | (a1, (GZeroOrMore g, a1r)), (a2, _)
   | (a2, _), (a1, (GZeroOrMore g, a1r)) ->
     assert (
-     Spec.array_group3_disjoint (Spec.maybe_close_array_group (array_group_sem e.e_sem_env a10) close) (Spec.maybe_close_array_group (array_group_sem e.e_sem_env a20) close) <==>
-       Spec.array_group3_disjoint (Spec.maybe_close_array_group (array_group_sem e.e_sem_env a1) close) (Spec.maybe_close_array_group (array_group_sem e.e_sem_env a2) close)
+     Spec.array_group_disjoint (Spec.maybe_close_array_group (array_group_sem e.e_sem_env a10) close) (Spec.maybe_close_array_group (array_group_sem e.e_sem_env a20) close) <==>
+       Spec.array_group_disjoint (Spec.maybe_close_array_group (array_group_sem e.e_sem_env a1) close) (Spec.maybe_close_array_group (array_group_sem e.e_sem_env a2) close)
      );
      let res1 = array_group_disjoint e fuel' close a1r a2 in
      if not (RSuccess? res1)
@@ -449,7 +508,7 @@ and array_group_disjoint
      else if RSuccess? (array_group_disjoint e fuel' false g a2) // loop-free shortcut, but will miss things like "disjoint? (a* ) (ab)"
      then RSuccess ()
      else begin
-       Spec.array_group3_concat_assoc (array_group_sem e.e_sem_env g) (array_group_sem e.e_sem_env (GZeroOrMore g)) (array_group_sem e.e_sem_env a1r);
+       Spec.array_group_concat_assoc (array_group_sem e.e_sem_env g) (array_group_sem e.e_sem_env (GZeroOrMore g)) (array_group_sem e.e_sem_env a1r);
        let a1' = GConcat g a1 in
        rewrite_group_correct e.e_sem_env fuel' a1';
        array_group_disjoint e fuel' close (rewrite_group fuel' _ a1') a2 // potential source of loops
@@ -457,8 +516,8 @@ and array_group_disjoint
    | (a1, (GOneOrMore g, a1r)), (a2, _)
    | (a2, _), (a1, (GOneOrMore g, a1r)) ->
      assert (
-       Spec.array_group3_disjoint (Spec.maybe_close_array_group (array_group_sem e.e_sem_env a10) close) (Spec.maybe_close_array_group (array_group_sem e.e_sem_env a20) close) <==>
-       Spec.array_group3_disjoint (Spec.maybe_close_array_group (array_group_sem e.e_sem_env a1) close) (Spec.maybe_close_array_group (array_group_sem e.e_sem_env a2) close)
+       Spec.array_group_disjoint (Spec.maybe_close_array_group (array_group_sem e.e_sem_env a10) close) (Spec.maybe_close_array_group (array_group_sem e.e_sem_env a20) close) <==>
+       Spec.array_group_disjoint (Spec.maybe_close_array_group (array_group_sem e.e_sem_env a1) close) (Spec.maybe_close_array_group (array_group_sem e.e_sem_env a2) close)
      );
      let a1' = GConcat (GConcat g (GZeroOrMore g)) a1r in
      rewrite_group_correct e.e_sem_env fuel' a1';
@@ -466,8 +525,8 @@ and array_group_disjoint
    | (a1, (GZeroOrOne g, a1r)), (a2, _)
    | (a2, _), (a1, (GZeroOrOne g, a1r)) ->
      assert (
-       Spec.array_group3_disjoint (Spec.maybe_close_array_group (array_group_sem e.e_sem_env a10) close) (Spec.maybe_close_array_group (array_group_sem e.e_sem_env a20) close) <==>
-       Spec.array_group3_disjoint (Spec.maybe_close_array_group (array_group_sem e.e_sem_env a1) close) (Spec.maybe_close_array_group (array_group_sem e.e_sem_env a2) close)
+       Spec.array_group_disjoint (Spec.maybe_close_array_group (array_group_sem e.e_sem_env a10) close) (Spec.maybe_close_array_group (array_group_sem e.e_sem_env a20) close) <==>
+       Spec.array_group_disjoint (Spec.maybe_close_array_group (array_group_sem e.e_sem_env a1) close) (Spec.maybe_close_array_group (array_group_sem e.e_sem_env a2) close)
      );
      let res = array_group_disjoint e fuel' close a1r a2 in
      if not (RSuccess? res)
@@ -570,7 +629,7 @@ let map_group_footprint_correct
     | Some ty, RSuccess t ->
       typ_bounded env.se_bound t /\
       ty `Spec.typ_equiv` typ_sem env t /\
-      MapSpec.map_group_footprint (map_group_sem env g) (typ_sem env t)
+      Spec.map_group_footprint (map_group_sem env g) (typ_sem env t)
     | _, RSuccess _ -> False
     | Some _, _ -> False
     | _ -> True
@@ -580,7 +639,7 @@ let map_group_footprint_correct
 = map_group_footprint_correct' env g;
   match spec_map_group_footprint env g, map_group_footprint g with
   | Some ty, RSuccess t ->
-    MapSpec.map_group_footprint_equiv (map_group_sem env g) ty (typ_sem env t)
+    Spec.map_group_footprint_equiv (map_group_sem env g) ty (typ_sem env t)
   | _ -> ()
 
 let coerce_failure
@@ -591,6 +650,7 @@ let coerce_failure
   | RFailure msg -> RFailure msg
   | ROutOfFuel -> ROutOfFuel
 
+(*
 #restart-solver
 let rec restrict_map_group
   (fuel: nat) // for typ_disjoint
@@ -606,7 +666,7 @@ let rec restrict_map_group
       match g' with
       | RSuccess g' ->
         group_bounded _ env.e_sem_env.se_bound g' /\
-        MapSpec.restrict_map_group
+        Spec.restrict_map_group
           (map_group_sem env.e_sem_env g)
           (map_group_sem env.e_sem_env g') /\
         begin match spec_map_group_footprint env.e_sem_env g, spec_map_group_footprint env.e_sem_env g' with
@@ -634,7 +694,7 @@ let rec restrict_map_group
       begin match restrict_map_group fuel env (left `TChoice` fp1) g2 with
       | RSuccess g2' ->
         let f2' = Ghost.hide (Some?.v (spec_map_group_footprint env.e_sem_env g2')) in
-        MapSpec.restrict_map_group_concat
+        Spec.restrict_map_group_concat
           (map_group_sem env.e_sem_env g1)
           (typ_sem env.e_sem_env fp1)
           (map_group_sem env.e_sem_env g1')
@@ -642,7 +702,7 @@ let rec restrict_map_group
           (map_group_sem env.e_sem_env g2')
           f2';
         let g' = GConcat g1' g2' in
-        assert (MapSpec.restrict_map_group
+        assert (Spec.restrict_map_group
           (map_group_sem env.e_sem_env g)
           (map_group_sem env.e_sem_env g')
         );
@@ -667,27 +727,29 @@ let rec restrict_map_group
   | GMapElem sq cut (TElem (ELiteral key)) value ->
     begin match typ_disjoint env fuel (TElem (ELiteral key)) left with
     | RSuccess _ ->
-      MapSpec.map_group_is_det_match_item_for
+      Spec.map_group_is_det_match_item_for
         cut
         (eval_literal key)
         (typ_sem env.e_sem_env value);
-      MapSpec.restrict_map_group_refl (map_group_sem env.e_sem_env g);
+      Spec.restrict_map_group_refl (map_group_sem env.e_sem_env g);
       RSuccess g
     | res -> coerce_failure res
     end
   | GZeroOrMore (GMapElem _ false key value) ->
     begin match typ_disjoint env fuel key left with
     | RSuccess _ ->
-      MapSpec.restrict_map_group_refl (map_group_sem env.e_sem_env g);
+      Spec.restrict_map_group_refl (map_group_sem env.e_sem_env g);
       RSuccess g
     | ROutOfFuel -> ROutOfFuel // the restriction heuristics should not depend on the fuel
     | _ ->
       RSuccess GNop
     end
   | _ -> RFailure "restrict_map_group: unsupported cases"
+*)
 
 #pop-options
 
+(*
 noeq
 type mk_wf_validate_map_group_t (left_elems: Spec.typ) (left_tables: Spec.typ) (g1: group NMapGroup) = {
   left_elems1: Spec.typ;
@@ -696,6 +758,7 @@ type mk_wf_validate_map_group_t (left_elems: Spec.typ) (left_tables: Spec.typ) (
   left_elems10: typ;
   left_tables10: typ;
 }
+*)
 
 let rec array_group_is_nonempty
   (fuel: nat) // to unfold definitions
@@ -704,7 +767,7 @@ let rec array_group_is_nonempty
 : Pure (result unit)
     (requires (group_bounded _ env.e_sem_env.se_bound g))
     (ensures fun r -> match r with
-    | RSuccess _ -> Spec.array_group3_is_nonempty (array_group_sem env.e_sem_env g)
+    | RSuccess _ -> Spec.array_group_is_nonempty (array_group_sem env.e_sem_env g)
     | _ -> True
     )
     (decreases fuel)
@@ -730,7 +793,7 @@ let rec array_group_is_nonempty
   | GArrayElem _ _
   | GAlwaysFalse -> RSuccess ()
 
-#push-options "--admit_smt_queries true" // "--z3rlimit 64 --split_queries always --query_stats --fuel 4 --ifuel 8"
+#push-options "--z3rlimit 64 --split_queries always --query_stats --fuel 4 --ifuel 8"
 
 #restart-solver
 let rec array_group_concat_unique_strong
@@ -745,7 +808,7 @@ let rec array_group_concat_unique_strong
       group_bounded _ env.e_sem_env.se_bound g2
     ))
     (ensures fun r -> match r with
-    | RSuccess _ -> Spec.array_group3_concat_unique_strong (array_group_sem env.e_sem_env g1) (array_group_sem env.e_sem_env g2)
+    | RSuccess _ -> Spec.array_group_concat_unique_strong (array_group_sem env.e_sem_env g1) (array_group_sem env.e_sem_env g2)
     | _ -> True
     )
     (decreases fuel)
@@ -761,7 +824,7 @@ let rec array_group_concat_unique_strong
     if not (RSuccess? res2)
     then res2
     else begin
-      Spec.array_group3_concat_unique_strong_choice_left
+      Spec.array_group_concat_unique_strong_choice_left
         (array_group_sem env.e_sem_env g1l)
         (array_group_sem env.e_sem_env g1r)
         (array_group_sem env.e_sem_env g2);
@@ -775,7 +838,7 @@ let rec array_group_concat_unique_strong
     if not (RSuccess? res2)
     then res2
     else begin
-      Spec.array_group3_concat_unique_strong_concat_left (array_group_sem env.e_sem_env g1l) (array_group_sem env.e_sem_env g1r) (array_group_sem env.e_sem_env g2);
+      Spec.array_group_concat_unique_strong_concat_left (array_group_sem env.e_sem_env g1l) (array_group_sem env.e_sem_env g1r) (array_group_sem env.e_sem_env g2);
       RSuccess ()
     end
   | WfAElem _ _ -> RSuccess ()
@@ -788,14 +851,14 @@ let rec array_group_concat_unique_strong
     begin match destruct_group g2 with
     | (GDef _ i, g2r) ->
       let g2' = GConcat (env.e_env i) g2r in
-      Spec.array_group3_concat_equiv
+      Spec.array_group_concat_equiv
         (env.e_sem_env.se_env i)
         (array_group_sem env.e_sem_env (env.e_env i))
         (array_group_sem env.e_sem_env g2r)
         (array_group_sem env.e_sem_env g2r);
       rewrite_group_correct env.e_sem_env fuel g2';
       let g22 = rewrite_group fuel _ g2' in
-      Spec.array_group3_concat_unique_strong_equiv
+      Spec.array_group_concat_unique_strong_equiv
         (array_group_sem env.e_sem_env g1)
         (array_group_sem env.e_sem_env g1)
         (array_group_sem env.e_sem_env g2)
@@ -816,12 +879,12 @@ let rec array_group_concat_unique_strong
         else begin
           match g1' with
           | GZeroOrMore _ ->
-            Spec.array_group3_concat_unique_strong_zero_or_more_left
+            Spec.array_group_concat_unique_strong_zero_or_more_left
               (array_group_sem env.e_sem_env g')
               (array_group_sem env.e_sem_env g2);
             RSuccess ()
           | GOneOrMore _ ->
-            Spec.array_group3_concat_unique_strong_one_or_more_left
+            Spec.array_group_concat_unique_strong_one_or_more_left
               (array_group_sem env.e_sem_env g')
               (array_group_sem env.e_sem_env g2);
             RSuccess ()          
@@ -834,14 +897,14 @@ let rec array_group_concat_unique_strong
         if not (RSuccess? res2)
         then res2
         else begin
-          Spec.array_group3_concat_unique_strong_zero_or_one_left
+          Spec.array_group_concat_unique_strong_zero_or_one_left
             (array_group_sem env.e_sem_env g')
             (array_group_sem env.e_sem_env g2);
-          assert (Spec.array_group3_concat_unique_strong
-            (Spec.array_group3_zero_or_one (array_group_sem env.e_sem_env g'))
+          assert (Spec.array_group_concat_unique_strong
+            (Spec.array_group_zero_or_one (array_group_sem env.e_sem_env g'))
             (array_group_sem env.e_sem_env g2)
           );
-          assert (Spec.array_group3_concat_unique_strong
+          assert (Spec.array_group_concat_unique_strong
             (array_group_sem env.e_sem_env g1)
             (array_group_sem env.e_sem_env g2)
           );
@@ -864,7 +927,7 @@ let rec array_group_concat_unique_weak
       spec_wf_array_group env.e_sem_env _ s2
     ))
     (ensures fun r -> match r with
-    | RSuccess _ -> Spec.array_group3_concat_unique_weak (array_group_sem env.e_sem_env g1) (array_group_sem env.e_sem_env g2)
+    | RSuccess _ -> Spec.array_group_concat_unique_weak (array_group_sem env.e_sem_env g1) (array_group_sem env.e_sem_env g2)
     | _ -> True
     )
     (decreases fuel)
@@ -880,7 +943,7 @@ let rec array_group_concat_unique_weak
     if not (RSuccess? res2)
     then res2
     else begin
-      Spec.array_group3_concat_unique_weak_choice_left
+      Spec.array_group_concat_unique_weak_choice_left
         (array_group_sem env.e_sem_env g1l)
         (array_group_sem env.e_sem_env g1r)
         (array_group_sem env.e_sem_env g2);
@@ -896,7 +959,7 @@ let rec array_group_concat_unique_weak
       if not (RSuccess? res2)
       then res2
       else begin
-        Spec.array_group3_concat_unique_weak_choice_right
+        Spec.array_group_concat_unique_weak_choice_right
           (array_group_sem env.e_sem_env g1)
           (array_group_sem env.e_sem_env g2l)
           (array_group_sem env.e_sem_env g2r);
@@ -938,12 +1001,12 @@ let rec array_group_concat_unique_weak
         else begin
           match g' with
           | GZeroOrMore _ ->
-            Spec.array_group3_concat_unique_weak_zero_or_more_left
+            Spec.array_group_concat_unique_weak_zero_or_more_left
               (array_group_sem env.e_sem_env g)
               (array_group_sem env.e_sem_env g2);
             RSuccess ()
           | GOneOrMore _ ->
-            Spec.array_group3_concat_unique_weak_one_or_more_left
+            Spec.array_group_concat_unique_weak_one_or_more_left
               (array_group_sem env.e_sem_env g)
               (array_group_sem env.e_sem_env g2);
             RSuccess ()
@@ -956,7 +1019,7 @@ let rec array_group_concat_unique_weak
         if not (RSuccess? res2)
         then res2
         else begin
-          Spec.array_group3_concat_unique_weak_zero_or_one_left
+          Spec.array_group_concat_unique_weak_zero_or_one_left
             (array_group_sem env.e_sem_env g)
             (array_group_sem env.e_sem_env g2);
           RSuccess ()
@@ -978,7 +1041,7 @@ let rec map_group_choice_compatible_no_cut
       spec_wf_parse_map_group env.e_sem_env _ s2
     ))
     (ensures fun r -> match r with
-    | RSuccess _ -> MapSpec.map_group_choice_compatible_no_cut (map_group_sem env.e_sem_env g1) (map_group_sem env.e_sem_env g2)
+    | RSuccess _ -> Spec.map_group_choice_compatible_no_cut (map_group_sem env.e_sem_env g1) (map_group_sem env.e_sem_env g2)
     | _ -> True
     )
     (decreases fuel)
@@ -987,13 +1050,13 @@ let rec map_group_choice_compatible_no_cut
   else let fuel' : nat = fuel - 1 in
   match s1 with
   | WfMLiteral false key value _ ->
-    MapSpec.map_group_choice_compatible_no_cut_match_item_for_no_cut
+    Spec.map_group_choice_compatible_no_cut_match_item_for_no_cut
       (eval_literal key)
       (typ_sem env.e_sem_env value)
       (map_group_sem env.e_sem_env g2);
     RSuccess ()
   | WfMZeroOrMore key value _ _ ->
-    MapSpec.map_group_choice_compatible_no_cut_zero_or_more_match_item_left
+    Spec.map_group_choice_compatible_no_cut_zero_or_more_match_item_left
       (typ_sem env.e_sem_env key)
       (typ_sem env.e_sem_env value)
       (map_group_sem env.e_sem_env g2);
@@ -1006,7 +1069,7 @@ let rec map_group_choice_compatible_no_cut
     if not (RSuccess? res2)
     then res2
     else begin
-      MapSpec.map_group_choice_compatible_no_cut_choice_left
+      Spec.map_group_choice_compatible_no_cut_choice_left
         (map_group_sem env.e_sem_env g1l)
         (map_group_sem env.e_sem_env g1r)
         (map_group_sem env.e_sem_env g2);
@@ -1017,7 +1080,7 @@ let rec map_group_choice_compatible_no_cut
     if not (RSuccess? res1)
     then res1
     else begin
-      MapSpec.map_group_choice_compatible_no_cut_zero_or_one_left
+      Spec.map_group_choice_compatible_no_cut_zero_or_one_left
         (map_group_sem env.e_sem_env g)
         (map_group_sem env.e_sem_env g2);
       RSuccess ()
@@ -1029,7 +1092,7 @@ let rec map_group_choice_compatible_no_cut
     if not (RSuccess? res1)
     then res1
     else begin
-      MapSpec.map_group_choice_compatible_no_cut_match_item_for_cut
+      Spec.map_group_choice_compatible_no_cut_match_item_for_cut
         (eval_literal key)
         (typ_sem env.e_sem_env value)
         (map_group_sem env.e_sem_env g2)
@@ -1044,7 +1107,7 @@ let rec map_group_choice_compatible_no_cut
     if not (RSuccess? res2)
     then res2
     else begin
-      MapSpec.map_group_choice_compatible_no_cut_concat_left
+      Spec.map_group_choice_compatible_no_cut_concat_left
         (map_group_sem env.e_sem_env g1l)
         (Some?.v (spec_map_group_footprint env.e_sem_env g1l))
         (map_group_sem env.e_sem_env g1r)
@@ -1067,7 +1130,7 @@ let rec map_group_choice_compatible
       spec_wf_parse_map_group env.e_sem_env _ s2
     ))
     (ensures fun r -> match r with
-    | RSuccess _ -> MapSpec.map_group_choice_compatible (map_group_sem env.e_sem_env g1) (map_group_sem env.e_sem_env g2)
+    | RSuccess _ -> Spec.map_group_choice_compatible (map_group_sem env.e_sem_env g1) (map_group_sem env.e_sem_env g2)
     | _ -> True
     )
     (decreases fuel)
@@ -1087,7 +1150,7 @@ let rec map_group_choice_compatible
     if not (RSuccess? res2)
     then res2
     else begin
-      MapSpec.map_group_choice_compatible_choice_left
+      Spec.map_group_choice_compatible_choice_left
         (map_group_sem env.e_sem_env g1l)
         (map_group_sem env.e_sem_env g1r)
         (map_group_sem env.e_sem_env g2);
@@ -1103,7 +1166,7 @@ let rec map_group_choice_compatible
       if not (RSuccess? res2)
       then res2
       else begin
-        MapSpec.map_group_choice_compatible_choice_right
+        Spec.map_group_choice_compatible_choice_right
           (map_group_sem env.e_sem_env g1)
           (map_group_sem env.e_sem_env g2l)
           (map_group_sem env.e_sem_env g2r);
@@ -1114,7 +1177,7 @@ let rec map_group_choice_compatible
       | WfMConcat g1l s1l g1r s1r ->
         begin match map_group_choice_compatible fuel' env s1l s2 with
         | RSuccess _ ->
-          MapSpec.map_group_choice_compatible_concat_left
+          Spec.map_group_choice_compatible_concat_left
             (map_group_sem env.e_sem_env g1l)
             (Some?.v (spec_map_group_footprint env.e_sem_env g1l))
             (map_group_sem env.e_sem_env g1r)
@@ -1130,7 +1193,7 @@ let rec map_group_choice_compatible
           if not (RSuccess? res2)
           then res2
           else begin
-            MapSpec.map_group_choice_compatible_concat_left
+            Spec.map_group_choice_compatible_concat_left
               (map_group_sem env.e_sem_env g1l)
               (Some?.v (spec_map_group_footprint env.e_sem_env g1l))
               (map_group_sem env.e_sem_env g1r)
@@ -1144,7 +1207,7 @@ let rec map_group_choice_compatible
         let RSuccess f2 = map_group_footprint g2 in
         begin match typ_disjoint env fuel (TElem (ELiteral key)) f2 with
         | RSuccess _ ->
-          MapSpec.map_group_choice_compatible_match_item_for cut (eval_literal key) (typ_sem env.e_sem_env value) (map_group_sem env.e_sem_env g2) (typ_sem env.e_sem_env f2);
+          Spec.map_group_choice_compatible_match_item_for cut (eval_literal key) (typ_sem env.e_sem_env value) (map_group_sem env.e_sem_env g2) (typ_sem env.e_sem_env f2);
           RSuccess ()
         | ROutOfFuel -> ROutOfFuel
         | RFailure _ ->
@@ -1159,7 +1222,7 @@ let rec map_group_choice_compatible
             if not (RSuccess? res2)
             then res2
             else begin
-              MapSpec.map_group_choice_compatible_match_item_for_concat_right
+              Spec.map_group_choice_compatible_match_item_for_concat_right
                 (eval_literal key)
                 (typ_sem env.e_sem_env value)
                 (map_group_sem env.e_sem_env g2l)
@@ -1173,20 +1236,21 @@ let rec map_group_choice_compatible
             if not (RSuccess? res1)
             then res1
             else begin
-              MapSpec.map_group_choice_compatible_match_item_for_zero_or_one_right cut (eval_literal key) (typ_sem env.e_sem_env value) (map_group_sem env.e_sem_env g);
+              Spec.map_group_choice_compatible_match_item_for_zero_or_one_right cut (eval_literal key) (typ_sem env.e_sem_env value) (map_group_sem env.e_sem_env g);
               RSuccess ()
             end
           | WfMLiteral cut2 key2 value2 _ ->
             if key <> key2
             then begin // this case should already have been eliminated by the typ_disjoint test above
-              MapSpec.map_group_choice_compatible_match_item_for cut (eval_literal key) (typ_sem env.e_sem_env value) (map_group_sem env.e_sem_env g2) (Spec.t_literal (eval_literal key2));
+              Classical.forall_intro_2 byte_seq_of_ascii_string_diff;
+              Spec.map_group_choice_compatible_match_item_for cut (eval_literal key) (typ_sem env.e_sem_env value) (map_group_sem env.e_sem_env g2) (Spec.t_literal (eval_literal key2));
               RSuccess ()
             end else begin
               let res1 = typ_disjoint env fuel value value2 in
               if not (RSuccess? res1)
               then res1
               else begin
-                MapSpec.map_group_choice_compatible_match_item_for_same
+                Spec.map_group_choice_compatible_match_item_for_same
                   (eval_literal key)
                   (typ_sem env.e_sem_env value)
                   (typ_sem env.e_sem_env value2)
@@ -1202,7 +1266,7 @@ let rec map_group_choice_compatible
 
 #pop-options
 
-#push-options "--admit_smt_queries true" // "--z3rlimit 128 --split_queries always --query_stats --fuel 4 --ifuel 8"
+#push-options "--z3rlimit 128 --split_queries always --query_stats --fuel 4 --ifuel 8"
 
 #restart-solver
 let rec mk_wf_typ
@@ -1228,20 +1292,25 @@ let rec mk_wf_typ
     | res -> coerce_failure res
     end
   | TMap m ->
+    let m2 = m in
+(*  
     begin match mk_wf_validate_map_group fuel' env Spec.t_always_false Spec.t_always_false (TElem EAlwaysFalse) (TElem EAlwaysFalse) m with
     | RSuccess s1 ->
       begin match restrict_map_group fuel env (TElem EAlwaysFalse) m with
       | RSuccess m2 ->
         rewrite_group_correct env.e_sem_env fuel m2;
         let m3 = rewrite_group fuel _ m2 in
-        begin match mk_wf_parse_map_group fuel' env m3 with
-        | RSuccess s3 -> RSuccess (WfTMap m _ _ s1.wf m3 s3)
+*)      
+        begin match mk_wf_parse_map_group fuel' env m with
+        | RSuccess s3 -> RSuccess (WfTMap m (* _ _ s1.wf m3 *) s3)
         | res -> coerce_failure res
         end
+(*
       | res -> coerce_failure res
-      end
+      end      
     | res -> coerce_failure res
     end
+*)
   | TTagged tag t' ->
     begin match mk_wf_typ fuel' env t' with
     | RSuccess s' -> RSuccess (WfTTagged tag t' s')
@@ -1381,13 +1450,14 @@ and mk_wf_parse_map_group
     | res -> coerce_failure res
     end
   | GZeroOrOne g' ->
-    begin match map_group_is_productive g' with
-    | RSuccess _ ->
-      map_group_is_productive_correct env.e_sem_env g';
+    begin match apply_map_group_det_empty_fail g' with
+    | RSuccess true ->
+      apply_map_group_det_empty_fail_correct env.e_sem_env g';
       begin match mk_wf_parse_map_group fuel' env g' with
       | RSuccess s' -> RSuccess (WfMZeroOrOne g' s')
       | res -> coerce_failure res
       end
+    | RSuccess _ -> RFailure "mk_wf_parse_map_group: group does not fail on empty"
     | res -> coerce_failure res
     end
   | GConcat g1 g2 ->
@@ -1415,6 +1485,7 @@ and mk_wf_parse_map_group
     end
   | _ -> RFailure "mk_wf_parse_map_group: unsupported"
 
+(*
 and mk_wf_validate_map_group
   (fuel: nat) // for typ_disjoint
   (env: ast_env)
@@ -1522,6 +1593,7 @@ and mk_wf_validate_map_group
     | res -> coerce_failure res
     end    
   | _ -> RFailure "mk_wf_validate_map_group: unsupported"
+*)
 
 #pop-options
 
@@ -1571,6 +1643,18 @@ let mk_wf_typ_fuel_for_intro
 : Tot (mk_wf_typ_fuel_for e t)
 = fuel
 
+unfold
+let wf_ast_env_extend_typ_with_weak_pre'
+  (e: wf_ast_env)
+  (new_name: string)
+  (t: typ)
+  (t_wf: ast0_wf_typ t)
+: Tot prop
+=
+    e.e_sem_env.se_bound new_name == None /\
+    typ_bounded e.e_sem_env.se_bound t /\
+    spec_wf_typ e.e_sem_env t t_wf
+
 [@@sem_attr]
 let compute_wf_typ
   (e: wf_ast_env)
@@ -1581,7 +1665,9 @@ let compute_wf_typ
 : Tot (t_wf: ast0_wf_typ t {
     wf_ast_env_extend_typ_with_weak_pre e new_name t t_wf
   })
-= RSuccess?._0 (mk_wf_typ' fuel e t)
+= let t_wf = RSuccess?._0 (mk_wf_typ' fuel e t) in
+  assert (wf_ast_env_extend_typ_with_weak_pre' e new_name t t_wf);
+  t_wf
 
 [@@sem_attr]
 let wf_ast_env_extend_typ
@@ -1595,7 +1681,9 @@ let wf_ast_env_extend_typ
       e'.e_sem_env.se_bound new_name == Some NType /\
       t == e'.e_env new_name
   })
-= wf_ast_env_extend_typ_with_weak e new_name t (RSuccess?._0 (mk_wf_typ' fuel e t))
+= let t_wf = RSuccess?._0 (mk_wf_typ' fuel e t) in
+  assert (wf_ast_env_extend_typ_with_weak_pre' e new_name t t_wf);
+  wf_ast_env_extend_typ_with_weak e new_name t t_wf
 
 exception ExceptionOutOfFuel
 
